Checkpoint switching to Z over nat for more stuff

new/proof/sync_proof/waitgroup.v
@@ -12,31 +12,32 @@ Local Definition waitGroupBubbleFlag := 2147483648.
 Example waitGroupBubbleFlag_ok : #waitGroupBubbleFlag = sync.waitGroupBubbleFlag :=
   eq_refl.
 
-Local Definition enc (low high : w32) : w64 :=
-  word.add (word.slu (W64 (uint.Z high)) (W64 32)) (W64 (uint.Z low)).
+Local Definition enc (wait counter : w32) : w64 :=
+  word.add (word.slu (W64 (uint.Z counter)) (W64 32)) (W64 (sint.Z wait)).
 
-Local Lemma enc_get_high (low high : w32) :
-  W32 (uint.Z (word.sru (enc low high) (W64 32))) = high.
+Local Lemma enc_get_counter (wait counter : w32) :
+  W32 (uint.Z (word.sru (enc wait counter) (W64 32))) = counter.
 Proof. unfold enc. word. Qed.
 
-Local Lemma enc_get_low (low high : w32) :
-  W32 (uint.Z (enc low high)) = low.
+Local Lemma enc_get_wait (wait counter : w32) :
+  0 ≤ sint.Z wait < 2^31 →
+  W32 (uint.Z (word.and (enc wait counter) (W64 2147483647))) = wait.
+Proof. unfold enc. admit. Admitted.
+
+Local Lemma enc_add_counter (wait counter delta : w32) :
+  word.add (enc wait counter) (word.slu (W64 (sint.Z delta)) (W64 32)) =
+  enc wait (word.add counter delta).
 Proof. unfold enc. word. Qed.
 
-Local Lemma enc_add_high (low high delta : w32) :
-  word.add (enc low high) (word.slu (W64 (sint.Z delta)) (W64 32)) =
-  enc low (word.add high delta).
+Local Lemma enc_add_wait (wait counter delta : w32) :
+  sint.Z (word.add wait delta) = sint.Z wait + sint.Z delta →
+  word.add (enc wait counter) (W64 (sint.Z delta)) =
+  enc (word.add wait delta) counter.
 Proof. unfold enc. word. Qed.
 
-Local Lemma enc_add_low (low high delta : w32) :
-  uint.Z (word.add low delta) = uint.Z low + sint.Z delta →
-  word.add (enc low high) (W64 (sint.Z delta)) =
-  enc (word.add low delta) high.
-Proof. unfold enc. word. Qed.
-
-Local Lemma enc_inj (low high low' high' : w32) :
-  enc low high = enc low' high' →
-  low = low' ∧ high = high'.
+Local Lemma enc_inj (wait counter wait' counter' : w32) :
+  enc wait counter = enc wait' counter' →
+  wait = wait' ∧ counter = counter'.
 Proof. unfold enc. intros. word. Qed.
 
 Local Lemma enc_0 :
@@ -52,8 +53,9 @@ Record WaitGroup_names := {
 
 Implicit Type γ : WaitGroup_names.
 
-Definition own_WaitGroup_waiters γ (possible_waiters : w32) : iProp Σ :=
-  own_tok_auth_dfrac γ.(waiter_gn) (DfracOwn (1/2)) (uint.nat possible_waiters).
+Definition own_WaitGroup_waiters γ (possible_waiters : Z) : iProp Σ :=
+  "%Hnonneg" ∷ ⌜ 0 ≤ possible_waiters ⌝ ∗
+  "Hpossible_waiters" ∷ own_tok_auth_dfrac γ.(waiter_gn) (DfracOwn (1/2)) (Z.to_nat possible_waiters).
 #[global] Opaque own_WaitGroup_waiters.
 #[local] Transparent own_WaitGroup_waiters.
 #[global] Instance own_WaitGroup_waiters_timeless γ w : Timeless (own_WaitGroup_waiters γ w) := _.
@@ -65,7 +67,7 @@ Definition own_WaitGroup_wait_token γ : iProp Σ :=
 #[global] Instance own_WaitGroup_wait_token_timeless γ  : Timeless (own_WaitGroup_wait_token γ) := _.
 
 Local Definition is_WaitGroup_inv wg γ N : iProp Σ :=
-  inv (N.@"wg") (∃ (counter waiters sema possible_waiters : w32) unfinished_waiters,
+  inv (N.@"wg") (∃ (counter waiters sema : w32) unfinished_waiters possible_waiters,
   "Hsema" ∷ own_sema γ.(sema_gn) sema ∗
   "Hsema_zerotoks" ∷  own_toks γ.(zerostate_gn) (uint.nat sema) ∗
 
@@ -77,18 +79,19 @@ Local Definition is_WaitGroup_inv wg γ N : iProp Σ :=
   "Hctr" ∷ ghost_var γ.(counter_gn) (1/2)%Qp counter ∗
 
   (* When Add's caller has [own_waiters 0], this resource implies that there are no waiters. *)
-  "Hwait_toks" ∷  own_toks γ.(waiter_gn) (uint.nat waiters) ∗
+  "Hwait_toks" ∷ own_toks γ.(waiter_gn) (sint.nat waiters) ∗
   "Hunfinished_wait_toks" ∷ own_toks γ.(waiter_gn) unfinished_waiters ∗
 
   "Hzeroauth" ∷ own_tok_auth γ.(zerostate_gn) unfinished_waiters ∗
 
-  (* keeping this to maintain that the number of waiters does not overflow. *)
-  "Hwaiters_bounded" ∷ own_tok_auth_dfrac γ.(waiter_gn) (DfracOwn (1/2)) (uint.nat possible_waiters) ∗
+  (* Keeping this to maintain that the number of waiters does not overflow. *)
+  "Hwaiters_bounded" ∷ own_tok_auth_dfrac γ.(waiter_gn) (DfracOwn (1/2)) possible_waiters ∗
+  "%Hpossible_waiters_bound" ∷ ⌜ Z.of_nat possible_waiters < 2^31 ⌝ ∗
 
   "%Hunfinished_zero" ∷ ⌜ unfinished_waiters ≠ O → waiters = W32 0 ∧ counter = W32 0 ⌝ ∗
-  "%Hunfinished_bound" ∷ ⌜ Z.of_nat unfinished_waiters < 2^32 ⌝
+  "%Hunfinished_bound" ∷ ⌜ Z.of_nat unfinished_waiters < 2^32 ⌝ ∗
+  "%Hwaiter_notbubbled" ∷ ⌜ 0 ≤ sint.Z waiters < 2^31 ⌝
   )%I.
-
 
 Definition is_WaitGroup wg γ N : iProp Σ :=
   "#Hsem" ∷ is_sema (struct_field_ref sync.WaitGroup.t "sema" wg) γ.(sema_gn) (N.@"sema") ∗
@@ -104,45 +107,43 @@ Instance if_sumbool_timeless {PROP : bi} (P Q : PROP) {_:Timeless P} {_:Timeless
 Proof. apply _. Qed.
 
 (* Prepare to Wait() *)
-Lemma alloc_wait_token wg γ N (w : w32) :
-  uint.Z (word.add w (W32 1)) = uint.Z w + 1 →
+Lemma alloc_wait_token wg γ N w :
+  0 < w + 1 < 2^31 →
   is_WaitGroup wg γ N -∗
-  own_WaitGroup_waiters γ w ={↑N}=∗ own_WaitGroup_waiters γ (word.add w (W32 1)) ∗ own_WaitGroup_wait_token γ.
+  own_WaitGroup_waiters γ w ={↑N}=∗ own_WaitGroup_waiters γ (w + 1) ∗ own_WaitGroup_wait_token γ.
 Proof.
-  intros H. iIntros "[_ #Hinv] H".
+  intros H. iIntros "[_ #Hinv] H". iNamed "H".
   iInv "Hinv" as ">Hi". iNamed "Hi".
-  iCombine "Hwaiters_bounded H" gives %[_ ->].
-  iCombine "Hwaiters_bounded H" as "H".
+  iCombine "Hwaiters_bounded Hpossible_waiters" gives %[_ ->].
+  iCombine "Hwaiters_bounded Hpossible_waiters" as "H".
   iMod (own_tok_auth_add 1 with "H") as "[H Htok]".
-  iModIntro. rewrite <- (Z2Nat.inj_add _ 1) by word. rewrite -H.
-  iDestruct "H" as "[H1 H2]". iSplitR "Htok H2"; by iFrame.
+  iModIntro. rewrite <- (Z2Nat.inj_add _ 1) by word.
+  iDestruct "H" as "[H1 H2]". iSplitR "Htok H2"; iFrame; word.
 Qed.
 
 Lemma waiters_none_token_false γ :
-  own_WaitGroup_waiters γ (W32 0) -∗ own_WaitGroup_wait_token γ -∗ False.
+  own_WaitGroup_waiters γ 0 -∗ own_WaitGroup_wait_token γ -∗ False.
 Proof.
-  iIntros "H1 H2".
-  iCombine "H1 H2" gives %H. word.
+  iIntros "H1 H2". iNamed "H1".
+  iCombine "Hpossible_waiters H2" gives %H. word.
 Qed.
 
-Lemma dealloc_wait_token wg γ N (w : w32) :
-  uint.Z (word.sub w (W32 1)) = uint.Z w - 1 →
+Lemma dealloc_wait_token wg γ N w :
+  0 ≤ w - 1 →
   is_WaitGroup wg γ N -∗
   own_WaitGroup_waiters γ w -∗
   own_WaitGroup_wait_token γ ={↑N}=∗
-  own_WaitGroup_waiters γ (word.sub w (W32 1)).
+  own_WaitGroup_waiters γ (w - 1).
 Proof.
-  intros H. iIntros "[_ #Hinv] H Htok".
+  intros H. iIntros "[_ #Hinv] H Htok". iNamed "H".
   iInv "Hinv" as ">Hi". iNamedSuffix "Hi" "_wg".
-  iCombine "Hwaiters_bounded_wg H" gives %[_ ->].
-  iCombine "Hwaiters_bounded_wg H" as "H".
+  iCombine "Hwaiters_bounded_wg Hpossible_waiters" gives %[_ ->].
+  iCombine "Hwaiters_bounded_wg Hpossible_waiters" as "H".
   iCombine "H Hunfinished_wait_toks_wg" gives %Hle.
   iMod (own_tok_auth_sub with "H Htok") as "[H Hwaiters_bounded_wg]".
   iModIntro. iFrame "∗#%".
-  replace (Z.to_nat (w32_word_instance.(word.unsigned) w) - 1)%nat with
-    (uint.nat (word.sub w (W32 1))).
-  2:{ word. }
-  by iFrame.
+  replace (Z.to_nat (w - 1)) with (Z.to_nat w - 1)%nat by word.
+  iFrame. word.
 Qed.
 
 Definition own_WaitGroup γ (counter : w32) : iProp Σ :=
@@ -154,7 +155,7 @@ Definition own_WaitGroup γ (counter : w32) : iProp Σ :=
 Lemma init_WaitGroup N wg_ptr :
   wg_ptr ↦ zero_val sync.WaitGroup.t ={⊤}=∗
   ∃ γ,
-  is_WaitGroup wg_ptr γ N ∗ own_WaitGroup γ (W32 0) ∗ own_WaitGroup_waiters γ (W32 0).
+  is_WaitGroup wg_ptr γ N ∗ own_WaitGroup γ (W32 0) ∗ own_WaitGroup_waiters γ 0.
 Proof.
   iIntros "H". iStructNamed "H". simpl.
 
@@ -193,8 +194,8 @@ Lemma wp_WaitGroup__Add (wg : loc) (delta : w64) γ N :
        "Hwg" ∷ own_WaitGroup γ oldc ∗
        "%Hbounds" ∷ ⌜ 0 ≤ sint.Z oldc + sint.Z delta' < 2^31 ⌝ ∗
        "HΦ" ∷ ((⌜ oldc ≠ W32 0 ⌝ ∗ (own_WaitGroup γ (word.add oldc delta') ={↑N,⊤}=∗ Φ #())) ∨
-         (own_WaitGroup_waiters γ (W32 0) ∗
-          (own_WaitGroup_waiters γ (W32 0) -∗ own_WaitGroup γ (word.add oldc delta') ={↑N,⊤}=∗
+         (own_WaitGroup_waiters γ 0 ∗
+          (own_WaitGroup_waiters γ 0 -∗ own_WaitGroup γ (word.add oldc delta') ={↑N,⊤}=∗
            Φ #())))
   ) -∗
   WP wg @! (go.PointerType sync.WaitGroup) @! "Add" #delta {{ Φ }}.
@@ -216,12 +217,13 @@ Proof.
     iExFalso.
     destruct Hw as [-> Hw].
     iDestruct "HΦ" as "[(% & _)|(HnoWaiter & HΦ)]"; first by exfalso.
+    iDestruct "HnoWaiter" as "[HnoWaiter _]".
     iCombine "HnoWaiter Hwait_toks_wg" gives %Hbad.
     exfalso. apply Hw. word.
   }
   iCombine "Hptsto_wg Hptsto2_wg" as "Hptsto".
   iExists _. iFrame.
-  rewrite (wg_delta_to_w32 delta') // enc_add_high.
+  rewrite (wg_delta_to_w32 delta') // enc_add_counter.
   iMod (ghost_var_update (word.add oldc delta') with "Hctr") as "[Hctr_wg Hwg]".
   iIntros "[Hptsto1_wg Hptsto2_wg]".
   destruct unfinished_waiters.
@@ -247,7 +249,12 @@ Proof.
       - iMod ("HΦ" with "[$] [$]"). done. }
     iModIntro.
     wp_auto.
-    rewrite enc_get_high enc_get_low.
+    wp_if_destruct.
+    2:{ word. }
+
+    rewrite enc_get_wait.
+    rewrite enc_get_counter.
+    enc_get_wait.
 
     destruct bool_decide eqn:Hbad.
     {
